HypeHeap now keeping track of dead regions

ulib/FStar.Monotonic.HyperHeap.fst
@@ -19,6 +19,12 @@ open FStar.Preorder
 open FStar.Monotonic.Heap
 module Set = FStar.Set
 
+
+
+(*+ Definition and properties of regions ids (rid) +*)
+
+(*! Definition of rid !*)
+
 abstract let rid = list (int * int)
 
 let reveal (r:rid) : GTot (list (int * int)) = r
@@ -28,14 +34,15 @@ abstract let color (x:rid): GTot int =
   | [] -> 0
   | (c, _)::_ -> c
 
-type t = Map.t rid heap
-
 let has_eq_rid (u:unit) :
   Lemma (requires True)
         (ensures hasEq rid)
   = ()
 
 assume HasEq_rid: hasEq rid //TODO: we just proved this above, but we need to expose it as an argument-free SMT lemma, which isn't supported yet
+
+
+(*! The root rid !*)
 
 abstract let root : rid = []
 
@@ -47,6 +54,151 @@ let lemma_root_has_color_zero r = ()
 
 //expose this so that no-one should assume otheriwse
 let root_has_color_zero (u:unit) :Lemma (color root == 0) = ()
+
+
+(*! Operations on rids !*)
+
+abstract val includes : rid -> rid -> GTot bool
+let rec includes r1 r2 =
+  if r1=r2 then true
+  else if List.Tot.length r2 > List.Tot.length r1
+  then includes r1 (Cons?.tl r2)
+  else false
+
+let disjoint (i:rid) (j:rid) : GTot bool =
+  not (includes i j) && not (includes j i)
+
+abstract val extends: rid -> rid -> GTot bool
+let extends r0 r1 = Cons? r0 && Cons?.tl r0 = r1
+
+abstract val parent: r:rid{r=!=root} -> Tot rid
+let parent r = Cons?.tl r
+
+let disjoint_regions (s1:Set.set rid) (s2:Set.set rid) : Tot Type0 =
+  forall x y. {:pattern (Set.mem x s1); (Set.mem y s2)} (Set.mem x s1 /\ Set.mem y s2) ==> disjoint x y
+
+(*! Lemmas on rid operations !*)
+
+abstract val lemma_includes_trans: i:rid -> j:rid -> k:rid ->
+  Lemma (requires (includes i j /\ includes j k))
+  (ensures (includes i k))
+  [SMTPat (includes i j); SMTPat (includes j k)]
+let rec lemma_includes_trans i j k =
+  if j=k then ()
+  else match k with
+    | hd::tl -> lemma_includes_trans i j tl
+
+abstract val lemma_includes_refl: i:rid ->
+  Lemma (requires (True))
+    (ensures (includes i i))
+    [SMTPat (includes i i)]
+let lemma_includes_refl i = ()
+
+abstract val lemma_extends_includes: i:rid -> j:rid ->
+  Lemma (requires (extends j i))
+    (ensures (includes i j /\ not(includes j i)))
+    [SMTPat (extends j i)]
+let lemma_extends_includes i j = ()
+
+let lemma_includes_anti_symmetric (i:rid) (j:rid) :
+  Lemma (requires (includes i j /\ i =!= j))
+    (ensures (not (includes j i)))
+    [SMTPat (includes i j)]
+= ()
+
+private
+val lemma_aux: k:rid -> i:rid ->
+  Lemma  (requires
+      List.Tot.length k > 0
+      /\ List.Tot.length k <= List.Tot.length i
+      /\ includes k i
+      /\ not (includes (Cons?.tl k) i))
+    (ensures False)
+    (decreases (List.Tot.length i))
+let rec lemma_aux k i = lemma_aux k (Cons?.tl i)
+
+abstract
+val lemma_disjoint_includes: i:rid -> j:rid -> k:rid ->
+  Lemma (requires (disjoint i j /\ includes j k))
+    (ensures (disjoint i k))
+    (decreases (List.Tot.length (reveal k)))
+    [SMTPat (disjoint i j); SMTPat (includes j k)]
+let rec lemma_disjoint_includes i j k =
+  if List.Tot.length k <= List.Tot.length j
+  then ()
+  else (lemma_disjoint_includes i j (Cons?.tl k);
+    if List.Tot.length i <= List.Tot.length (Cons?.tl k)
+    then ()
+    else if includes k i
+    then lemma_aux k i
+    else ())
+
+
+abstract
+val lemma_extends_disjoint: i:rid -> j:rid -> k:rid ->
+  Lemma (requires (extends j i /\ extends k i /\ j=!=k))
+    (ensures (disjoint j k))
+let lemma_extends_disjoint i j k = ()
+
+abstract
+val lemma_extends_parent: i:rid{i=!=root} ->
+  Lemma (requires True)
+    (ensures (extends i (parent i)))
+    [SMTPat (parent i)]
+let lemma_extends_parent i = ()
+
+abstract
+val lemma_extends_not_root: i:rid -> j:rid{extends j i} ->
+  Lemma (requires True)
+    (ensures (j=!=root))
+    [SMTPat (extends j i)]
+let lemma_extends_not_root i j = ()
+
+abstract
+val lemma_extends_only_parent: i:rid -> j:rid{extends j i} ->
+  Lemma (requires True)
+    (ensures (i = parent j))
+    [SMTPat (extends j i)]
+let lemma_extends_only_parent i j = ()
+
+abstract
+val lemma_disjoint_parents: pr:rid -> r:rid -> ps:rid -> s:rid ->
+  Lemma
+    (requires (r `extends` pr /\ s `extends` ps /\ disjoint pr ps))
+    (ensures (disjoint r s))
+    [SMTPat (extends r pr); SMTPat (extends s ps); SMTPat (disjoint pr ps)]
+let lemma_disjoint_parents pr r ps s =
+  assert (pr `includes` r);
+  assert (ps `includes` s)
+
+abstract
+val lemma_include_cons: i:rid -> j:rid ->
+  Lemma (requires (i=!=j /\ includes i j))
+    (ensures (j=!=root))
+let lemma_include_cons i j = ()
+
+let extends_parent (tip:rid{tip=!=root}) (r:rid)
+  : Lemma (requires True)
+    (extends r (parent tip) /\ r=!=tip ==> disjoint r tip \/ extends r tip)
+    [SMTPat (extends r (parent tip))]
+= ()
+
+let includes_child (tip:rid{tip=!=root}) (r:rid)
+  : Lemma (requires True)
+    (includes r tip ==> r==tip \/ includes r (parent tip))
+    [SMTPat (includes r (parent tip))]
+= ()
+
+let root_is_root (s:rid)
+  : Lemma (requires (includes s root))
+    (ensures (s == root))
+    [SMTPat (includes s root)]
+= ()
+
+private let test0 = assert (includes [(0, 1) ; (1, 0)] [(2, 2); (0, 1); (1, 0)])
+private let test1 (r1:rid) (r2:rid{includes r1 r2}) = assert (includes r1 ((0,0)::r2))
+
+(*+ Definition of monotonic region-based reference (mrref) +*)
 
 abstract type mrref (id:rid) (a:Type) (rel:preorder a) = mref a rel
 
@@ -63,162 +215,106 @@ val addr_of: #a:Type -> #id:rid -> #rel:preorder a -> r:mrref id a rel -> GTot n
 let addr_of #a #id #rel r = addr_of (as_ref r)
 
 let is_mm (#a:Type) (#id:rid) (#rel:preorder a) (r:mrref id a rel) :GTot bool
-  = is_mm (as_ref r)
+= is_mm (as_ref r)
 
 abstract val ref_as_rref : #a:Type -> #rel:preorder a -> i:rid -> r:mref a rel -> GTot (mrref i a rel)
 let ref_as_rref #a #rel i r = r
 
 val lemma_as_ref_inj: #a:Type -> #i:rid -> #rel:preorder a -> r:mrref i a rel
-    -> Lemma (requires (True))
-             (ensures ((ref_as_rref i (as_ref r) == r)))
-       [SMTPat (as_ref r)]
+-> Lemma (requires (True))
+(ensures ((ref_as_rref i (as_ref r) == r)))
+[SMTPat (as_ref r)]
 let lemma_as_ref_inj #a #i #rel r = ()
 
-abstract val includes : rid -> rid -> GTot bool
-let rec includes r1 r2 =
-  if r1=r2 then true
-  else if List.Tot.length r2 > List.Tot.length r1
-  then includes r1 (Cons?.tl r2)
-  else false
+(*+ Definition of HyperHeap (t) +*)
 
-let disjoint (i:rid) (j:rid) : GTot bool =
-  not (includes i j) && not (includes j i)
+noeq
+type maybe_live_heap = | H : live:bool -> m:heap -> maybe_live_heap
 
-private val lemma_aux: k:rid -> i:rid
-      -> Lemma  (requires
-                    List.Tot.length k > 0
-                    /\ List.Tot.length k <= List.Tot.length i
-                    /\ includes k i
-                    /\ not (includes (Cons?.tl k) i))
-                 (ensures False)
-                 (decreases (List.Tot.length i))
-let rec lemma_aux k i = lemma_aux k (Cons?.tl i)
+type t = Map.t rid maybe_live_heap
 
-abstract val lemma_disjoint_includes: i:rid -> j:rid -> k:rid ->
-  Lemma (requires (disjoint i j /\ includes j k))
-        (ensures (disjoint i k))
-        (decreases (List.Tot.length (reveal k)))
-        [SMTPat (disjoint i j);
-         SMTPat (includes j k)]
-let rec lemma_disjoint_includes i j k =
-  if List.Tot.length k <= List.Tot.length j
-  then ()
-  else (lemma_disjoint_includes i j (Cons?.tl k);
-        if List.Tot.length i <= List.Tot.length (Cons?.tl k)
-        then ()
-        else (if includes k i
-              then lemma_aux k i
-              else ()))
+let contains (m:t) (i:rid) : Tot bool = Map.contains m i && (Map.sel m i).live
+let at (m:t) (i:rid{ m `contains` i}) : Tot heap = (Map.sel m i).m
 
-abstract val extends: rid -> rid -> GTot bool
-let extends r0 r1 = Cons? r0 && Cons?.tl r0 = r1
-
-abstract val parent: r:rid{r=!=root} -> Tot rid
-let parent r = Cons?.tl r
-
-abstract val lemma_includes_refl: i:rid
-                      -> Lemma (requires (True))
-                               (ensures (includes i i))
-                               [SMTPat (includes i i)]
-let lemma_includes_refl i = ()
-
-abstract val lemma_extends_includes: i:rid -> j:rid ->
-  Lemma (requires (extends j i))
-        (ensures (includes i j /\ not(includes j i)))
-        [SMTPat (extends j i)]
-let lemma_extends_includes i j = ()
-
-let lemma_includes_anti_symmetric (i:rid) (j:rid) :
-  Lemma (requires (includes i j /\ i =!= j))
-        (ensures (not (includes j i)))
-        [SMTPat (includes i j)]
-  = ()
-
-abstract val lemma_extends_disjoint: i:rid -> j:rid -> k:rid ->
-    Lemma (requires (extends j i /\ extends k i /\ j=!=k))
-          (ensures (disjoint j k))
-let lemma_extends_disjoint i j k = ()
-
-abstract val lemma_extends_parent: i:rid{i=!=root} ->
-  Lemma (requires True)
-        (ensures (extends i (parent i)))
-        [SMTPat (parent i)]
-let lemma_extends_parent i = ()
-
-abstract val lemma_extends_not_root: i:rid -> j:rid{extends j i} ->
-  Lemma (requires True)
-        (ensures (j=!=root))
-        [SMTPat (extends j i)]
-let lemma_extends_not_root i j = ()
-
-abstract val lemma_extends_only_parent: i:rid -> j:rid{extends j i} ->
-  Lemma (requires True)
-        (ensures (i = parent j))
-        [SMTPat (extends j i)]
-let lemma_extends_only_parent i j = ()
-
-private let test0 = assert (includes [(0, 1) ; (1, 0)] [(2, 2); (0, 1); (1, 0)])
-private let test1 (r1:rid) (r2:rid{includes r1 r2}) = assert (includes r1 ((0,0)::r2))
-
-let fresh_region (i:rid) (m0:t) (m1:t) =
+let fresh_region (i:rid) (m0:t) (m1:t) : Tot Type0 =
+ (* No child region can be contained in the previous heap (even dead) *)
  (forall j. includes i j ==> not (Map.contains m0 j))
- /\ Map.contains m1 i
+ (* and the region `i` is contained in the new heap *)
+ /\ m1 `contains` i
+
 
 (* KM : surprisingly, using the Tot version makes an assert fail in HyperStack... to be investigated *)
-let contains_ref_tot (#a:Type) (#rel:preorder a) (#i:rid) (m:t) (r:mrref i a rel) : Type0 =
-  Map.contains m i /\ Map.sel m i `Heap.contains` r
+let contains_ref (#a:Type) (#rel:preorder a) (#i:rid) (m:t) (r:mrref i a rel) : Tot Type0 =
+  m `contains` i /\ (m `at` i) `Heap.contains` (as_ref r)
 
-let contains_ref (#a:Type) (#rel:preorder a) (#i:rid) (m:t) (r:mrref i a rel) :GTot bool  =
-  Map.contains m i && (FStar.StrongExcludedMiddle.strong_excluded_middle (Heap.contains (Map.sel m i) (as_ref r)))
+let contains_ref_bool (#a:Type) (#rel:preorder a) (#i:rid) (m:t) (r:mrref i a rel) :GTot bool  =
+  m `contains` i &&
+  FStar.StrongExcludedMiddle.strong_excluded_middle ((m `at` i) `Heap.contains` (as_ref r))
 
-let unused_in_tot (#a:Type) (#rel:preorder a) (#i:rid) (r:mrref i a rel) (m:t) :Tot Type0 =
-  ~(Map.contains m i) \/ Heap.unused_in (as_ref r) (Map.sel m i)
+let unused_in (#a:Type) (#rel:preorder a) (#i:rid) (r:mrref i a rel) (m:t) :Tot Type0 =
+  ~(m `contains` i) \/ Heap.unused_in (as_ref r) (m `at` i)
 
-let unused_in (#a:Type) (#rel:preorder a) (#i:rid) (r:mrref i a rel) (m:t) :GTot bool =
-not (Map.contains m i) ||
-FStar.StrongExcludedMiddle.strong_excluded_middle (Heap.unused_in (as_ref r) (Map.sel m i))
+let unused_in_bool (#a:Type) (#rel:preorder a) (#i:rid) (r:mrref i a rel) (m:t) :GTot bool =
+  not (m `contains` i) ||
+  FStar.StrongExcludedMiddle.strong_excluded_middle (Heap.unused_in (as_ref r) (m `at` i))
 
-let weak_contains_ref_tot (#a:Type) (#rel:preorder a) (#i:rid) (r:mrref i a rel) (m:t) : Tot Type0 =
-Heap.contains (Map.sel m i) r
+(* KM : Do we really not want to assert anything about the liveness of the heap ? *)
+let weak_contains_ref (#a:Type) (#rel:preorder a) (#i:rid) (m:t) (r:mrref i a rel) : Tot Type0 =
+  Heap.contains (Map.sel m i).m (as_ref r)
 
-let weak_contains_ref (#a:Type) (#rel:preorder a) (#i:rid) (r:mrref i a rel) (m:t) : GTot bool =
-FStar.StrongExcludedMiddle.strong_excluded_middle (Heap.contains (Map.sel m i) (as_ref r))
+let weak_contains_ref_bool (#a:Type) (#rel:preorder a) (#i:rid) (m:t) (r:mrref i a rel) : GTot bool =
+    FStar.StrongExcludedMiddle.strong_excluded_middle (weak_contains_ref m r)
 
+let fresh_rref (#a:Type) (#rel:preorder a) (#i:rid) (r:mrref i a rel) (m0:t) (m1:t) =
+  r `unused_in` m0 /\ m1 `contains_ref` r
+
+
+(*+ Accessing and mutating the heap +*)
 
 let sel_tot (#a:Type) (#rel:preorder a) (#i:rid) (m:t) (r:mrref i a rel{m `contains_ref` r})
   : Tot a
-= sel_tot (Map.sel m i) (as_ref r)
+= sel_tot (m `at` i) (as_ref r)
 
-let sel (#a:Type) (#rel:preorder a) (#i:rid) (m:t) (r:mrref i a rel) : GTot a
-  = sel (Map.sel m i) (as_ref r)
+let sel (#a:Type) (#rel:preorder a) (#i:rid) (m:t) (r:mrref i a rel)
+  : GTot a
+= sel (Map.sel m i).m (as_ref r)
 unfold let op_String_Access (#a:Type) (#rel:preorder a) (#i:rid) (m:t) (r:mrref i a rel) = sel m r
 
 
 let upd_tot (#a:Type) (#rel:preorder a) (#i:rid) (m:t) (r:mrref i a rel{m `contains_ref` r}) (v:a{rel (sel m r) v})
   : Tot t
-= Map.upd m i (upd_tot (Map.sel m i) (as_ref r) v)
+= Map.upd m i (H true (upd_tot (m `at` i) (as_ref r) v))
 
-let upd (#a:Type) (#rel:preorder a) (#i:rid) (m:t) (r:mrref i a rel) (v:a{rel (sel m r) v}) :GTot t
-  = Map.upd m i (upd (Map.sel m i) (as_ref r) v)
+let upd (#a:Type) (#rel:preorder a) (#i:rid) (m:t) (r:mrref i a rel) (v:a{rel (sel m r) v})
+  : GTot t
+= let hm = Map.sel m i in
+  Map.upd m i (H hm.live (upd hm.m (as_ref r) v))
 unfold let op_String_Assignment (#a:Type) (#rel:preorder a) (#i:rid) (m:t) (r:mrref i a rel) v = upd m r v
 
-let alloc (id:rid) (#a:Type0) (rel:preorder a) (m:t) (init:a) (mm:bool) : Tot (mrref id a rel * t) =
-  let (r, h) : mref a rel * heap = alloc rel (Map.sel m id) init mm in
-  r, Map.upd m id h
+let alloc (id:rid) (#a:Type0) (rel:preorder a) (m:t{m `contains` id}) (init:a) (mm:bool) : Tot (mrref id a rel * t) =
+  let (r, h) : mref a rel * heap = alloc rel (m `at` id) init mm in
+  r, Map.upd m id (H true h)
 
-let free_mm (#a:Type0) (#id:rid) (#rel:preorder a) (m:t) (r:mrref id a rel{m `contains_ref` r /\ is_mm r}) : GTot t =
-  let h0 = Map.sel m id in
+let free_mm (#a:Type0) (#id:rid) (#rel:preorder a) (m:t) (r:mrref id a rel{m `contains_ref` r /\ is_mm r}) : Tot t =
+  let h0 = m `at` id in
   let h1 = Heap.free_mm h0 (as_ref r) in
-  Map.upd m id h1
+  Map.upd m id (H true h1)
 
-abstract
-let free_mm_tot (#a:Type0) (#id:rid) (#rel:preorder a) (m:t) (r:mrref id a rel{m `contains_ref` r /\ is_mm r}) : Tot t =
-  let h0 = Map.sel m id in
-  let h1 = Heap.free_mm h0 r in
-  Map.upd m id h1
+let lemma_alloc (id:rid) (#a:Type0) (rel:preorder a) (m0:t) (init:a) (mm:bool)
+  : Lemma (requires (m0 `contains` id))
+    (ensures (
+      m0 `contains` id /\
+      (let r, m1 = alloc id rel m0 init mm in
+        fresh_rref r m0 m1 /\
+        rel (sel m0 r) init /\
+        m1 == upd m0 r init /\
+        is_mm r == mm)))
+= Heap.lemma_alloc rel (m0 `at` id) init mm
 
-let lemma_free_mm_coincides (#a:Type0) (#id:rid) (#rel:preorder a) (m:t) (r:mrref id a rel{m `contains_ref` r /\ is_mm r}) : Lemma (free_mm m r == free_mm_tot m r) = ()
 
+(*+ Modifies clauses on hyperheaps +*)
+
+(* Downward closure of a set of rids *)
 assume val mod_set : Set.set rid -> Tot (Set.set rid)
 assume Mod_set_def: forall (x:rid) (s:Set.set rid). {:pattern Set.mem x (mod_set s)}
                     Set.mem x (mod_set s) <==> (exists (y:rid). Set.mem y s /\ includes y x)
@@ -250,16 +346,6 @@ abstract val lemma_modifies_trans: m1:t -> m2:t -> m3:t
                                (ensures (modifies (Set.union s1 s2) m1 m3))
 let lemma_modifies_trans m1 m2 m3 s1 s2 = ()
 
-abstract val lemma_includes_trans: i:rid -> j:rid -> k:rid
-                        -> Lemma (requires (includes i j /\ includes j k))
-                                 (ensures (includes i k))
-                                 [SMTPat (includes i j);
-                                  SMTPat (includes j k)]
-let rec lemma_includes_trans i j k =
-  if j=k then ()
-  else match k with
-        | hd::tl -> lemma_includes_trans i j tl
-
 abstract val lemma_modset: i:rid -> j:rid
                   -> Lemma (requires (includes j i))
                            (ensures (Set.subset (mod_set (Set.singleton i)) (mod_set (Set.singleton j))))
@@ -277,81 +363,30 @@ abstract val lemma_modifies_includes2: m1:t -> m2:t
                                 (ensures (modifies s2 m1 m2))
 let lemma_modifies_includes2 m1 m2 s1 s2 = ()
 
-abstract val lemma_disjoint_parents: pr:rid -> r:rid -> ps:rid -> s:rid -> Lemma
-  (requires (r `extends` pr /\ s `extends` ps /\ disjoint pr ps))
-  (ensures (disjoint r s))
-  [SMTPat (extends r pr); SMTPat (extends s ps); SMTPat (disjoint pr ps)]
-let lemma_disjoint_parents pr r ps s =
-    assert (pr `includes` r);
-    assert (ps `includes` s)
-
-let fresh_rref (#a:Type) (#rel:preorder a) (#i:rid) (r:mrref i a rel) (m0:t) (m1:t) =
-  FStar.Monotonic.Heap.unused_in (as_ref r) (Map.sel m0 i) /\
-  FStar.Monotonic.Heap.contains (Map.sel m1 i) (as_ref r)
-
-let lemma_alloc (id:rid) (#a:Type0) (rel:preorder a) (m0:t) (init:a) (mm:bool)
-  : Lemma (requires True)
-    (ensures (
-      let r, m1 = alloc id rel m0 init mm in
-      fresh_rref r m0 m1 /\ rel (sel m0 r) init /\ m1 == upd m0 r init /\ is_mm r == mm
-    ))
-= Heap.lemma_alloc rel (Map.sel m0 id) init mm
 
 let modifies_rref (r:rid) (s:Set.set nat) h0 h1 =
   Heap.modifies s (Map.sel h0 r) (Map.sel h1 r)
 
-abstract val lemma_include_cons: i:rid -> j:rid -> Lemma
-  (requires (i=!=j /\ includes i j))
-  (ensures (j=!=root))
-let lemma_include_cons i j = ()
-
+(*+ Upward closedness of the map and related lemmas +*)
 let map_invariant (m:t) =
   forall r. Map.contains m r ==>
       (forall s. includes s r ==> Map.contains m s)
 
-abstract val lemma_extends_fresh_disjoint: i:rid -> j:rid -> ipar:rid -> jpar:rid
-                               -> m0:t{map_invariant m0} -> m1:t{map_invariant m1} ->
-  Lemma (requires (fresh_region i m0 m1
-                  /\ fresh_region j m0 m1
-                  /\ Map.contains m0 ipar
-                  /\ Map.contains m0 jpar
-                  /\ extends i ipar
-                  /\ extends j jpar
-                  /\ i=!=j))
-        (ensures (disjoint i j))
-        [SMTPatT (fresh_region i m0 m1);
-         SMTPatT (fresh_region j m0 m1);
-         SMTPat (extends i ipar);
-         SMTPat (extends j jpar)]
+abstract
+val lemma_extends_fresh_disjoint:
+  i:rid -> j:rid -> ipar:rid -> jpar:rid ->
+  m0:t{map_invariant m0} -> m1:t{map_invariant m1} ->
+  Lemma (requires (
+      fresh_region i m0 m1
+      /\ fresh_region j m0 m1
+      /\ m0 `contains` ipar
+      /\ m0 `contains` jpar
+      /\ extends i ipar
+      /\ extends j jpar
+      /\ i=!=j))
+    (ensures (disjoint i j))
+    [SMTPatT (fresh_region i m0 m1);
+      SMTPatT (fresh_region j m0 m1);
+      SMTPat (extends i ipar);
+      SMTPat (extends j jpar)]
 let lemma_extends_fresh_disjoint i j ipar jpar m0 m1 = ()
-
-let disjoint_regions (s1:Set.set rid) (s2:Set.set rid) =
-     forall x y. {:pattern (Set.mem x s1); (Set.mem y s2)} (Set.mem x s1 /\ Set.mem y s2) ==> disjoint x y
-
-let extends_parent (tip:rid{tip=!=root}) (r:rid)
-  : Lemma (requires True)
-          (extends r (parent tip) /\ r=!=tip ==> disjoint r tip \/ extends r tip)
-          [SMTPat (extends r (parent tip))]
-  = ()
-
-let includes_child (tip:rid{tip=!=root}) (r:rid)
-  : Lemma (requires True)
-          (includes r tip ==> r==tip \/ includes r (parent tip))
-          [SMTPat (includes r (parent tip))]
-  = ()
-
-let root_is_root (s:rid)
-  : Lemma (requires (includes s root))
-          (ensures (s == root))
-          [SMTPat (includes s root)]
-  = ()
-
-let lemma_sel_equals_sel_tot_for_contained_refs
-  (#a:Type) (#i:rid) (#rel:preorder a) (m:t) (r:mrref i a rel{m `contains_ref` r})
-  : Lemma (ensures (sel_tot m r == sel m r))
-= ()
-
-let lemma_upd_equals_upd_tot_for_contained_refs
-  (#a:Type) (#i:rid) (#rel:preorder a) (m:t) (r:mrref i a rel{m `contains_ref` r}) (v:a{rel (sel m r) v})
-  : Lemma (ensures (upd_tot m r v == upd m r v))
-= ()
